Change the type of fspec using Prop: remove meta

imp_system/mem/MemA.v
@@ -229,7 +229,7 @@ Module MemP. Section MemP.
   Definition scopes := ["Mem"].
 
   (* Function specifications *)
-  Definition fnsems : alist (option string) (fnsem_type (option fspec * fbody)) :=
+  Definition fnsems : alist (option string) (fnsem_type (option fspec_rel * fbody)) :=
   [(Some MemHdr.alloc, (false, wmask_all, scopes, (None, lat_real false MemSpec.alloc (Ret ()) fbody_trivial)));
    (Some MemHdr.free,  (false, wmask_all, scopes, (None, lat_real false MemSpec.free  (Ret ()) fbody_trivial)));
    (Some MemHdr.load,  (false, wmask_all, scopes, (None, lat_real false MemSpec.load  (Ret ()) fbody_trivial)));
@@ -256,22 +256,22 @@ Module MemA. Section MemA.
 
   Definition scopes := ["Mem"].
 
-  Definition sp : alist (option string) (option fspec) :=
+  Definition sp : alist (option string) (option fspec_rel) :=
     Seal.sealing CRIS
-      [(Some MemHdr.alloc, Some (to_fspec MemSpec.alloc));
-       (Some MemHdr.free,  Some (to_fspec MemSpec.free));
-       (Some MemHdr.load,  Some (to_fspec MemSpec.load));
-       (Some MemHdr.store, Some (to_fspec MemSpec.store));
-       (Some MemHdr.cmp,   Some (to_fspec MemSpec.cmp));
-       (Some MemHdr.cas,   Some (to_fspec MemSpec.cas))].
+      [(Some MemHdr.alloc, Some (to_fspec MemSpec.alloc: fspec_rel));
+       (Some MemHdr.free,  Some (to_fspec MemSpec.free: fspec_rel));
+       (Some MemHdr.load,  Some (to_fspec MemSpec.load: fspec_rel));
+       (Some MemHdr.store, Some (to_fspec MemSpec.store: fspec_rel));
+       (Some MemHdr.cmp,   Some (to_fspec MemSpec.cmp: fspec_rel));
+       (Some MemHdr.cas,   Some (to_fspec MemSpec.cas: fspec_rel))].
 
-  Definition fnsems : alist (option string) (fnsem_type (option fspec * fbody)) :=
-    [(Some MemHdr.alloc, (true, wmask_all, scopes, (Some (to_fspec MemSpec.alloc), fbody_trivial)));
-     (Some MemHdr.free,  (true, wmask_all, scopes, (Some (to_fspec MemSpec.free), fbody_trivial)));
-     (Some MemHdr.load,  (true, wmask_all, scopes, (Some (to_fspec MemSpec.load), fbody_trivial)));
-     (Some MemHdr.store, (true, wmask_all, scopes, (Some (to_fspec MemSpec.store), fbody_trivial)));
-     (Some MemHdr.cmp,   (true, wmask_all, scopes, (Some (to_fspec MemSpec.cmp), fbody_trivial)));
-     (Some MemHdr.cas,   (true, wmask_all, scopes, (Some (to_fspec MemSpec.cas), fbody_trivial)))].
+  Definition fnsems : alist (option string) (fnsem_type (option fspec_rel * fbody)) :=
+    [(Some MemHdr.alloc, (true, wmask_all, scopes, (Some (to_fspec MemSpec.alloc: fspec_rel), fbody_trivial)));
+     (Some MemHdr.free,  (true, wmask_all, scopes, (Some (to_fspec MemSpec.free: fspec_rel), fbody_trivial)));
+     (Some MemHdr.load,  (true, wmask_all, scopes, (Some (to_fspec MemSpec.load: fspec_rel), fbody_trivial)));
+     (Some MemHdr.store, (true, wmask_all, scopes, (Some (to_fspec MemSpec.store: fspec_rel), fbody_trivial)));
+     (Some MemHdr.cmp,   (true, wmask_all, scopes, (Some (to_fspec MemSpec.cmp: fspec_rel), fbody_trivial)));
+     (Some MemHdr.cas,   (true, wmask_all, scopes, (Some (to_fspec MemSpec.cas: fspec_rel), fbody_trivial)))].
 
   (* Module definition *)
   Program Definition smod : SMod.t := {|
