theories/cancellation/CancelPost.v
@@ -3,7 +3,7 @@ Require Import LMod LModTr GSim GSimFacts GSimTactics.
 Require Import MInline MInlineIntro MInlineElim ElimRel.
 
 Lemma cancel_post `{Σ: GRA} md sp:
-  ∀ (rs0 : Σ) r_s r_t srcs tgts cid st ps pt vret X X' x x' Qo Qo' itrS ktrT k rs_diff
+  ∀ (rs0 : Σ) r_s r_t srcs tgts cid st ps pt vret Qo Qo' itrS ktrT k rs_diff
     (r : ∀ x x0, (x→x0→Prop)→smj→smj→itree coreE x→itree coreE x0→Prop)
     (WFS: SMod.wf md)
     (VP: valid_sp md sp)
@@ -34,16 +34,16 @@ Lemma cancel_post `{Σ: GRA} md sp:
     (LEN : cid < length srcs)
     (x2 : rs_diff !! cid = Some ε)
     (x0 : srcs !! cid = Some (ModTr.trans (tau;; tau;; itrS)))
-    (x1 : tgts !! cid = Some (x <- ModTr.trans (x <- elim_postcond Qo Qo' x x' vret;; ktrT x);; k x))
+    (x1 : tgts !! cid = Some (x <- ModTr.trans (x <- elim_postcond Qo Qo' vret;; ktrT x);; k x))
     (RET : cid = 0 → k = λ x : Any.t, Ret x)
     (KTR :
-    ∃ Q : X → Any.t → Any.t → iProp Σ,
+    ∃ Q : Any.t → Any.t → iProp Σ,
       (Qo = Some Q
-       ∨ Qo = None ∧ Q = λ (_ : X) (varg arg : Any.t), ⌜varg = arg⌝%I)
-      ∧ ∃ Q' : X' → Any.t → Any.t → iProp Σ,
+       ∨ Qo = None ∧ Q = λ (varg arg : Any.t), ⌜varg = arg⌝%I)
+      ∧ ∃ Q' : Any.t → Any.t → iProp Σ,
           (Qo' = Some Q'
-           ∨ Qo' = None ∧ Q' = λ (_ : X') (varg arg : Any.t), ⌜varg = arg⌝%I)
-          ∧ (∀ ret : Any.t, Q' x' vret ret ⊢ |==> Q x vret ret)
+           ∨ Qo' = None ∧ Q' = λ (varg arg : Any.t), ⌜varg = arg⌝%I)
+          ∧ (∀ ret : Any.t, Q' vret ret ⊢ |==> Q vret ret)
             ∧ upaco4 (elim_rel_def sp) bot4 Any.t ε itrS (ktrT vret)),
 
   gpaco7 _gsim (cpn7 _gsim) bot7 r (Any.t * Any.t)%type 
@@ -72,7 +72,7 @@ Proof.
       ziter_r. zstep_r. eexists r_t. zstep_r.
       ziter_r. zstep_r. unshelve eexists.
       { split; [eapply Own_wand_valid; [iIntros "S"; iMod (RS with "S") as "[_ $]"|]|]; try done.
-        iIntros "H". iMod (x6 with "H") as "[P O]". rewrite KTR1. iFrame. 
+        iIntros "H". iMod (x5 with "H") as "[P O]". rewrite KTR1. iFrame. 
       }
       zstep_r.
       ziter_r. zstep_r. ziter_r. zstep_r. ziter_r. zstep_r.
@@ -81,14 +81,14 @@ Proof.
       { rewrite list_insert_id //. }
       { econs; eauto; eapply KTR1. }
     }
-    { assert (vret = x3).
+    { assert (vret = x).
       { eapply Own_pure_soundness; try apply WFR.
-        rewrite RS. iIntros ">[? H]". iMod (x6 with "H") as "[P O]".
+        rewrite RS. iIntros ">[? H]". iMod (x5 with "H") as "[P O]".
         rewrite KTR1. iMod "P" as "P"; et.
       }
       des. subst.
       ired. pclearbot. eapply KEY; et.
-      rewrite RS list_insert_id //. iIntros ">[$ H]". iMod (x6 with "H") as "[P O]". iFrame. et.
+      rewrite RS list_insert_id //. iIntros ">[$ H]". iMod (x5 with "H") as "[P O]". iFrame. et.
       econs; eauto; eapply KTR1.
     }
   }
